implement cmpxchg / atomicrmw for sequential memory (#398)
* implement cmpxchg for sequential memory

* add partial support for atomicrmw instructions

* implement nand for atomicrmw

* LangRefine proofs for cmpxchg and atomicrmw.

---------

Co-authored-by: Calvin Beck <hobbes@ualberta.ca>

tests/ll/atomicrmw.ll
@@ -1,0 +1,104 @@
+;; Compare and swap when the values stored/compared are i32s
+define i32 @atomicrmw_i32_add(i32 %x, i32 %y) {
+   %ptr = alloca i32
+   store i32 %x, ptr %ptr
+   %ans = atomicrmw add ptr %ptr, i32 %y acq_rel
+   %res = load i32, ptr %ptr
+   ret i32 %res
+}
+
+; ASSERT EQ: i32 42 = call i32 @atomicrmw_i32_add(i32 17, i32 25)
+; ASSERT EQ: i32 100 = call i32 @atomicrmw_i32_add(i32 10, i32 90)
+
+
+;; Compare and swap when the values stored/compared are i32s
+define i32 @atomicrmw_i32_sub(i32 %x, i32 %y) {
+   %ptr = alloca i32
+   store i32 %x, ptr %ptr
+   %ans = atomicrmw sub ptr %ptr, i32 %y acq_rel
+   %res = load i32, ptr %ptr
+   ret i32 %res
+}
+
+; ASSERT EQ: i32 8 = call i32 @atomicrmw_i32_sub(i32 25, i32 17)
+; ASSERT EQ: i32 80 = call i32 @atomicrmw_i32_sub(i32 90, i32 10)
+
+
+;; Compare and swap when the values stored/compared are i32s
+define i32 @atomicrmw_i32_xchg(i32 %x, i32 %y) {
+   %ptr = alloca i32
+   store i32 %x, ptr %ptr
+   %ans = atomicrmw xchg ptr %ptr, i32 %y acq_rel
+   %res = load i32, ptr %ptr
+   ret i32 %res
+}
+
+; ASSERT EQ: i32 17 = call i32 @atomicrmw_i32_xchg(i32 25, i32 17)
+; ASSERT EQ: i32 10 = call i32 @atomicrmw_i32_xchg(i32 90, i32 10)
+
+
+;; Compare and swap when the values stored/compared are i32s
+define i32 @atomicrmw_i32_and(i32 %x, i32 %y) {
+   %ptr = alloca i32
+   store i32 %x, ptr %ptr
+   %ans = atomicrmw and ptr %ptr, i32 %y acq_rel
+   %res = load i32, ptr %ptr
+   ret i32 %res
+}
+
+; ASSERT EQ: i32 17 = call i32 @atomicrmw_i32_and(i32 25, i32 17)
+; ASSERT EQ: i32 16 = call i32 @atomicrmw_i32_and(i32 25, i32 16)
+
+
+;; Compare and swap when the values stored/compared are i32s
+define i32 @atomicrmw_i32_or(i32 %x, i32 %y) {
+   %ptr = alloca i32
+   store i32 %x, ptr %ptr
+   %ans = atomicrmw or ptr %ptr, i32 %y acq_rel
+   %res = load i32, ptr %ptr
+   ret i32 %res
+}
+
+; ASSERT EQ: i32 27 = call i32 @atomicrmw_i32_or(i32 24, i32 11)
+; ASSERT EQ: i32 25 = call i32 @atomicrmw_i32_or(i32 25, i32 16)
+
+;; Compare and swap when the values stored/compared are i32s
+define i32 @atomicrmw_i32_xor(i32 %x, i32 %y) {
+   %ptr = alloca i32
+   store i32 %x, ptr %ptr
+   %ans = atomicrmw xor ptr %ptr, i32 %y acq_rel
+   %res = load i32, ptr %ptr
+   ret i32 %res
+}
+
+; ASSERT EQ: i32 19 = call i32 @atomicrmw_i32_xor(i32 24, i32 11)
+; ASSERT EQ: i32 9 = call i32 @atomicrmw_i32_xor(i32 25, i32 16)
+
+
+
+;; Compare and swap when the values stored/compared are i5s
+define i5 @atomicrmw_i5_nand(i5 %x, i5 %y) {
+   %ptr = alloca i5
+   store i5 %x, ptr %ptr
+   %ans = atomicrmw nand ptr %ptr, i5 %y acq_rel
+   %res = load i5, ptr %ptr
+   ret i5 %res
+}
+
+; ASSERT EQ: i5 23 = call i5 @atomicrmw_i5_nand(i5 24, i5 11)
+; ASSERT EQ: i5 22 = call i5 @atomicrmw_i5_nand(i5 15, i5 9)
+
+
+;; Compare and swap when the values stored/compared are i8s
+define i8 @atomicrmw_i8_nand(i8 %x, i8 %y) {
+   %ptr = alloca i8
+   store i8 %x, ptr %ptr
+   %ans = atomicrmw nand ptr %ptr, i8 %y acq_rel
+   %res = load i8, ptr %ptr
+   ret i8 %res
+}
+
+; ASSERT EQ: i8 127 = call i8 @atomicrmw_i8_nand(i8 255, i8 128)
+
+
+
