src/rocq/Semantics/Denotation.v
@@ -435,6 +435,131 @@ Module Denotation (LP : LLVMParams) (MP : MemoryParams LP) (Byte : ByteModule LP
   Definition catch_llvm_exc_L0' : itree L0' ~> eitherT uvalue (itree L0')
       := interp_either catch_llvm_exc_L0'_h.
 
+  Definition denote_cmpxchg id cpx : itree instr_E unit :=
+    (* SAZ: This will have to be revisited when we have a truly concurrent semantics. *)
+    let '(ptr_ty, ptr_val) := cpx.(c_ptr) in
+    let '(cmp_ty, cmp_val) := cpx.(c_cmp) in
+    let '(new_ty, new_val) := cpx.(c_new) in
+
+    (* Check whether the comparison types agree.  LLVM IR requires them to be integer
+           or pointer types (otherwise the IR is not well formed).  Vellvm checks that
+           the types are the same, but doesn't check their specific type.
+     *)
+    if (dtyp_eq_dec cmp_ty new_ty) then
+      
+      (* evaluate the arguments to the instruction *)
+      ptr_uv <- translate exp_to_instr (denote_exp (Some ptr_ty) ptr_val) ;;
+      cmp_uv <- translate exp_to_instr (denote_exp' (Some cmp_ty) cmp_val) ;;
+      new_uv <- translate exp_to_instr (denote_exp' (Some cmp_ty) new_val) ;;
+      
+      (* Perform the load - load addresses must be unique *)
+      ptr_dv <- concretize_or_pick_unique ptr_uv;;
+      loaded_uv <- trigger (Load cmp_ty ptr_dv);;
+
+      (* Perform the comparison - again we have to concretize the results *)
+      dv <- concretize_or_pick_unique (UVALUE_ICmp Eq loaded_uv cmp_uv);;
+      match dv with
+      | @DVALUE_I 1 comparison_bit =>
+          if equ comparison_bit one then
+            
+            (* They compared as equal: perform the write to memory *)
+            trigger (Store cmp_ty ptr_dv new_uv) ;;
+            (* return a struct with the loaded value and "true" *)
+            let ret_uv := UVALUE_Struct [loaded_uv; @UVALUE_I 1 one] in
+            trigger (LocalWrite id ret_uv);;
+            ret tt
+          else
+            (* They compared as distinct: do not perform the write to memory *)
+            (* return a struct with the loaded value and "false" *)                
+            let ret_uv := UVALUE_Struct [loaded_uv; @UVALUE_I 1 zero] in
+            trigger (LocalWrite id ret_uv);;
+            ret tt
+      | DVALUE_Poison dt => raiseUB "comparing poison in atomiccmpxchg."
+      | _ => raise "Br got non-bool value"
+      end
+    else 
+      raise "Ill-typed atomiccmpxchg".
+
+
+  (* Implement the atomic modify operations in terms of Vellvm uvalues.
+     Note: Langref doesn't seem to specifiy whether the arithmetic operations should be treated
+           as having (or not) the signed/wrapping flags activated.  Here we (arbitrarily?)
+           set them to false.
+  *)
+  Definition denote_atomic_rmw_operation a_op (pv : uvalue) (val : uvalue) : itree instr_E uvalue :=
+    match a_op with      
+    | Axchg =>
+        (* xchg: *ptr = val *)
+        ret val   
+    | Aadd =>
+        (* add: *ptr = *ptr + val *)
+        ret (UVALUE_IBinop (Add false false) pv val)
+    | Asub =>
+        (* sub: *ptr = *ptr - val *)
+        ret (UVALUE_IBinop (Sub false false) pv val)
+    | Aand =>
+        (* and: *ptr = *ptr - val *)
+        ret (UVALUE_IBinop And pv val)
+    | Aor =>
+        (* or: *ptr = *ptr | val *)
+        ret (UVALUE_IBinop Or pv val)
+    | Axor =>
+        (* xor: *ptr = *ptr ^ val *)
+        ret (UVALUE_IBinop Xor pv val)
+    | Anand =>
+        (* nand: *ptr = ~( *ptr & val ) *)
+        match val with
+        | UVALUE_I sz _ =>
+            (* SAZ: Is this the best way to get a UValue with 0xFFFF..FFFF bit pattern? *)
+            ret (UVALUE_IBinop (Sub false false)
+                   (@UVALUE_I sz (@repr (@bit_int sz) _ (@max_unsigned (@bit_int sz) _)))
+                   (UVALUE_IBinop And pv val))            
+        | _ => raise "atomicrmw nand of non-integer value"
+        end
+    | Afadd =>
+        (* fadd: *ptr = *ptr + val (using floating point arithmetic) *)
+        ret (UVALUE_FBinop FAdd [] pv val)
+    | Afsub =>
+        (* fsub: *ptr = *ptr - val (using floating point arithmetic) *)
+        ret (UVALUE_FBinop FSub [] pv val)
+    | Amax
+    | Amin
+    | Aumax
+    | Aumin
+    | Afmax
+    | Afmin
+    | Afmaximum
+    | Afminimum
+    | Auinc_wrap
+    | Audec_wrap
+    | Ausub_cond
+    | Ausub_sat => raise "Unsupported atomicrwm operation"
+    end.
+    
+  
+  Definition denote_atomicrmw id armw : itree instr_E unit :=
+    let '(ptr_ty, ptr_val) := armw.(a_ptr) in
+    let '(a_ty, a_val) := armw.(a_val) in
+    let a_op := armw.(a_operation) in
+
+    (* evaluate the arguments to the instruction *)
+    ptr_uv <- translate exp_to_instr (denote_exp (Some ptr_ty) ptr_val) ;;
+    a_uv <- translate exp_to_instr (denote_exp' (Some a_ty) a_val) ;;
+    
+    (* Perform the load - load addresses must be unique *)
+    ptr_dv <- concretize_or_pick_unique ptr_uv;;
+    loaded_uv <- trigger (Load a_ty ptr_dv);;
+
+    stored_uv <- denote_atomic_rmw_operation a_op loaded_uv a_uv ;;
+
+    (* Perform the store *)
+    trigger (Store a_ty ptr_dv stored_uv) ;;
+    
+    (* The result is the original value loaded from ptr before the modification *)
+    trigger (LocalWrite id loaded_uv);;
+    ret tt.
+
+  
   (* An instruction has only side-effects, it therefore returns [unit] *)
   Definition denote_instr
     (i: (instr_id * instr dtyp * list (metadata dtyp))) (varargs : option ADDR.addr) : itree instr_E unit :=
@@ -576,14 +701,18 @@ Module Denotation (LP : LLVMParams) (MP : MemoryParams LP) (Byte : ByteModule LP
         | IId id  => trigger (LocalWrite id retv);;
                      ret tt
         end
-    | (_, INSTR_LandingPad _ _ _) => raise "todo landingpad"
-    (* Currently unhandled itree instructions *)
-    | (_, INSTR_Fence _ _)
-    | (_, INSTR_AtomicCmpXchg _)
-    | (_, INSTR_AtomicRMW _) => raise "Unsupported VIR instruction"
+          
+    | (IId id, INSTR_AtomicCmpXchg cpx) =>
+        denote_cmpxchg id cpx
 
+    | (IId id, INSTR_AtomicRMW armw) =>
+        denote_atomicrmw id armw
+                       
+    (* Currently unhandled itree instructions *)
+    | (_, INSTR_LandingPad _ _ _) => raise "Unsupported INSTR_Landingpad"
+    | (_, INSTR_Fence _ _) => raise "Unsupported INSTR_Fence"
     (* Error states *)
-    | (_, _) => raise "ID / Instr mismatch void/non-void"
+    | (_, _) => raise "ID / Instr mismatch void / non-void"
     end.
 
   (* Computes the label to be returned by a switch terminator, after evaluation of values
